Dexter2 lqt (#2)

execution/examples/Dexter2FA12.v
@@ -1,4 +1,4 @@
-From Coq Require Import ZArith.
+From Coq Require Import ZArith Bool Lia.
 From Coq Require Import Morphisms.
 Require Import Monads.
 Require Import Extras.
@@ -69,7 +69,9 @@ Record State :=
 
 Record Setup :=
   build_setup {
-    admin_ : Address
+    admin_ : Address;
+    lqt_provider : Address;
+    initial_pool : N
 }.
 
 (* Any contract that wants to receive callback messages from the FA1.2 liquidity contract
@@ -213,10 +215,10 @@ Definition try_get_total_supply (sender : Address) (param : getTotalSupply_param
 
 Definition init (chain : Chain) (ctx : ContractCallContext) (setup : Setup) : option State :=
   Some {|
-    tokens := FMap.empty;
+    tokens := FMap.add setup.(lqt_provider) setup.(initial_pool) FMap.empty;
     allowances := FMap.empty;
     admin := setup.(admin_);
-    total_supply := 0
+    total_supply := setup.(initial_pool);
   |}.
 
 Open Scope Z_scope.
@@ -226,7 +228,7 @@ Definition receive (chain : Chain) (ctx : ContractCallContext)
   let sender := ctx.(ctx_from) in
   let without_actions := option_map (fun new_state => (new_state, [])) in
   let without_statechange acts := Some (state, acts) in
-  if ctx.(ctx_amount) >? 0
+  if 0 <? ctx.(ctx_amount)
   then None (* DontSendTez *)
   else match maybe_msg with
   | Some (msg_transfer param) => without_actions (try_transfer sender param state)
@@ -239,4 +241,1005 @@ Definition receive (chain : Chain) (ctx : ContractCallContext)
   end.
 Close Scope Z_scope.
 
+Definition contract : Contract Setup Msg State :=
+  build_contract init receive.
+
+
+
+Section Theories.
+
+(* receive only returns Some if the sender amount is zero *)
+Lemma contract_not_payable : forall prev_state new_state chain ctx msg new_acts,
+  receive chain ctx prev_state msg = Some (new_state, new_acts) ->
+    ((ctx_amount ctx) <= 0)%Z.
+Proof.
+  intros * receive_some.
+  unfold receive in receive_some.
+  destruct_match eqn:amount in receive_some.
+  - (* case: ctx_amount > 0 *)
+    congruence.
+  - (* case: ctx_amount <= 0 *)
+    now rewrite Z.ltb_ge in amount.
+Qed.
+
+Lemma contract_not_payable' : forall prev_state chain ctx msg,
+  (0 < (ctx_amount ctx))%Z ->
+    receive chain ctx prev_state msg = None.
+Proof.
+  intros * ctx_amount_positive.
+  unfold receive.
+  destruct_match eqn:amount.
+  - (* case: ctx_amount > 0 *)
+    reflexivity.
+  - (* case: ctx_amount <= 0 *)
+    now apply Z.ltb_ge in amount.
+Qed.
+
+Ltac receive_simpl_step :=
+  match goal with
+  | H : Blockchain.receive _ _ _ _ _ = Some (_, _) |- _ =>
+      unfold Blockchain.receive in H; cbn in H
+  | H : receive _ _ _ _ = Some (_, _) |- _ =>
+      apply contract_not_payable in H as ctx_amount_zero;
+      apply Z.ltb_ge in ctx_amount_zero;
+      unfold receive in H;
+      rewrite ctx_amount_zero in H;
+      cbn in H
+  | |- receive _ _ _ _ = _ =>
+      unfold receive; cbn
+  | H : Some _ = Some _ |- _ =>
+      inversion_clear H
+  | H : Some _ = None |- _ =>
+      inversion H
+  | H : None = Some _ |- _ =>
+      inversion H
+  | H : returnIf _ = None |- _ =>
+    let G := fresh "G" in
+      unfold returnIf in H;
+      destruct_match eqn:G in H; try congruence;
+      clear H;
+      rename G into H
+  | H : returnIf _ = Some ?u |- _ =>
+    let G := fresh "G" in
+      unfold returnIf in H;
+      destruct_match eqn:G in H; try congruence;
+      clear H u;
+      rename G into H
+  | H : option_map (fun s : State => (s, _)) match ?m with | Some _ => _ | None => None end = Some _ |- _ =>
+    let a := fresh "H" in
+    destruct m eqn:a in H; try setoid_rewrite a; cbn in *; try congruence
+  | H : option_map (fun s : State => (s, _)) (if ?m then ?a else ?b) = Some _ |- _ =>
+    match a with
+    | None =>
+      let a := fresh "H" in
+      destruct m eqn:a in H; try setoid_rewrite a; cbn in *; try congruence
+    | _ => match b with
+           | None =>
+             let a := fresh "H" in
+             destruct m eqn:a in H; try setoid_rewrite a; cbn in *; try congruence
+           | _ => idtac
+    end end
+  | H : (if ?m then ?a else ?b) = Some _ |- _ =>
+    match a with
+    | None =>
+      let a := fresh "H" in
+      destruct m eqn:a in H; try setoid_rewrite a; cbn in *; try congruence
+    | _ => match b with
+           | None =>
+             let a := fresh "H" in
+             destruct m eqn:a in H; try setoid_rewrite a; cbn in *; try congruence
+           | _ => idtac
+    end end
+  end.
+
+Tactic Notation "receive_simpl" := repeat receive_simpl_step.
+
+
+
+(* ------------------- Admin is constant ------------------- *)
+
+(* admin cannot be changed *)
+Lemma admin_constant : forall prev_state new_state chain ctx new_acts msg,
+  receive chain ctx prev_state msg = Some (new_state, new_acts) ->
+    admin prev_state = admin new_state.
+Proof.
+  intros * receive_some.
+  receive_simpl.
+  destruct msg. destruct m.
+  all : now receive_simpl.
+Qed.
+
+
+
+(* ------------------- Default entrypoint correct ------------------- *)
+
+(* Default entrypoint should never succeed *)
+Lemma default_entrypoint_none : forall prev_state chain ctx,
+  receive chain ctx prev_state None = None.
+Proof.
+  intros *.
+  receive_simpl.
+  now destruct_match.
+Qed.
+
+
+
+(* ------------------- Transfer correct ------------------- *)
+
+Definition transfer_balance_update_correct old_state new_state from to amount :=
+  let get_balance addr state := with_default 0 (FMap.find addr state.(tokens)) in
+  let from_balance_before := get_balance from old_state in
+  let to_balance_before := get_balance to old_state in
+  let from_balance_after := get_balance from new_state in
+  let to_balance_after := get_balance to new_state in
+  (* if the transfer is a self-transfer, balances should remain unchained *)
+  if address_eqb from to
+  then
+    (from_balance_before =? from_balance_after) &&
+    (to_balance_before =? to_balance_after)
+  else
+    (from_balance_before =? from_balance_after + amount) &&
+    (to_balance_before + amount =? to_balance_after).
+
+(* try_transfer correctly moves <amount> from <from> to <to> *)
+Lemma try_transfer_balance_correct : forall prev_state new_state chain ctx new_acts param,
+  receive chain ctx prev_state (Some (msg_transfer param)) = Some (new_state, new_acts) ->
+  transfer_balance_update_correct prev_state new_state param.(from) param.(to) param.(value) = true.
+Proof.
+  intros * receive_some.
+  receive_simpl.
+  rename H1 into enough_balance.
+  rewrite N.ltb_ge in enough_balance.
+  unfold transfer_balance_update_correct.
+  cbn.
+  destruct_match eqn:from_to_eqb.
+  - (* from = to *)
+    destruct (address_eqb_spec param.(from) param.(to)) as [<-|]; auto.
+    rewrite !FMap.find_add.
+    cbn.
+    rewrite !N.sub_add; auto.
+    now setoid_rewrite N.eqb_refl.
+  - (* from <> to *)
+    destruct (address_eqb_spec param.(from) param.(to)) as [| from_to_eq]; auto.
+    rewrite FMap.find_add_ne; auto.
+    rewrite ?FMap.find_add.
+    rewrite FMap.find_add_ne; auto.
+    cbn.
+    rewrite !N.sub_add; auto.
+    now setoid_rewrite N.eqb_refl.
+Qed.
+
+Definition transfer_allowances_update_correct old_state new_state sender from amount :=
+  let get_allowance addr1 addr2 state := with_default 0 (FMap.find (addr1, addr2) state.(allowances)) in
+  let allowance_before := get_allowance from sender old_state in
+  let allowance_after := get_allowance from sender new_state in
+  (* if the from and sender is equal, allowances should remain unchained *)
+  if address_eqb sender from
+  then
+    (allowance_before =? allowance_after)
+  else
+    (allowance_before =? allowance_after + amount).
+
+(* try_transfer correctly subtracts <amount> from allowances if <sender> is not <from> *)
+Lemma try_transfer_allowance_correct : forall prev_state new_state chain ctx new_acts param,
+  receive chain ctx prev_state (Some (msg_transfer param)) = Some (new_state, new_acts) ->
+  transfer_allowances_update_correct prev_state new_state ctx.(ctx_from) param.(from) param.(value) = true.
+Proof.
+  intros * receive_some.
+  receive_simpl.
+  clear g0 H1.
+  unfold transfer_allowances_update_correct.
+  cbn.
+  destruct_match eqn:sender_from_eqb.
+  - (* sender = from *)
+    rename H into allowances_eq.
+    inversion_clear allowances_eq.
+    now rewrite N.eqb_refl.
+  - (* sender <> from *)
+    receive_simpl.
+    rename H0 into enough_allowance.
+    rewrite N.ltb_ge in enough_allowance.
+    rewrite FMap.find_add.
+    cbn.
+    rewrite N.sub_add; auto.
+    now rewrite N.eqb_refl.
+Qed.
+
+(* try_transfer does not produce any new actions *)
+Lemma try_transfer_new_acts_correct : forall prev_state new_state chain ctx new_acts param,
+  receive chain ctx prev_state (Some (msg_transfer param)) = Some (new_state, new_acts) ->
+    new_acts = [].
+Proof.
+  intros * receive_some.
+  receive_simpl.
+Qed.
+
+(* try_transfer does not change the total supply of tokens *)
+Lemma try_transfer_preserves_total_supply : forall prev_state new_state chain ctx new_acts param,
+  receive chain ctx prev_state (Some (msg_transfer param)) = Some (new_state, new_acts) ->
+    total_supply prev_state = total_supply new_state.
+Proof.
+  intros * receive_some.
+  receive_simpl.
+Qed.
+
+(* try_transfer only modifies the <from> and <to> balances *)
+Lemma try_transfer_preserves_other_balances : forall prev_state new_state chain ctx new_acts param,
+  receive chain ctx prev_state (Some (msg_transfer param)) = Some (new_state, new_acts) ->
+    forall account, account <> param.(from) -> account <> param.(to) ->
+      FMap.find account (tokens prev_state) = FMap.find account (tokens new_state).
+Proof.
+  intros * receive_some account account_not_from account_not_to.
+  receive_simpl.
+  cbn.
+  rewrite !FMap.find_add_ne; auto.
+Qed.
+
+(* try_transfer only modifies the <sender> and <from> allowances *)
+Lemma try_transfer_preserves_other_allowances : forall prev_state new_state chain ctx new_acts param,
+  receive chain ctx prev_state (Some (msg_transfer param)) = Some (new_state, new_acts) ->
+    forall allowance_key, allowance_key <> (param.(from), ctx.(ctx_from)) ->
+      FMap.find allowance_key (allowances prev_state) = FMap.find allowance_key (allowances new_state).
+Proof.
+  intros * receive_some account allowance_key_ne.
+  receive_simpl.
+  cbn.
+  rename H into allowance_eq.
+  destruct_address_eq.
+  - (* from = sender *)
+    now inversion_clear allowance_eq.
+  - (* from <> sender *)
+    destruct_match in allowance_eq;
+      inversion_clear allowance_eq;
+      rewrite !FMap.find_add_ne; auto.
+Qed.
+
+(* If the requirements are met then then receive on transfer msg must succeed and
+    if receive on transfer msg succeeds then requirements must hold *)
+Lemma try_transfer_is_some : forall state chain ctx param,
+  (ctx_amount ctx <= 0)%Z /\
+  param.(value) <= with_default 0 (FMap.find param.(from) (tokens state)) /\
+  (param.(from) <> ctx.(ctx_from) ->
+    param.(value) <= with_default 0 (FMap.find (param.(from), ctx.(ctx_from)) (allowances state)))
+    <-> exists new_state new_acts, receive chain ctx state (Some (msg_transfer param)) = Some (new_state, new_acts).
+Proof.
+  split.
+  - intros (amount_zero & enough_balance & enough_allowance).
+    (*do 2 eexists.
+    receive_simpl.*)
+    unfold receive.
+    apply Z.ltb_ge in amount_zero.
+    rewrite amount_zero.
+    cbn.
+    destruct_match eqn:allowances_eq;
+    destruct_match eqn:sender_from_eqb in allowances_eq; try congruence;
+    try destruct_match eqn:enough_allowance_check in allowances_eq; try congruence;
+    try destruct_match eqn:new_balance;
+    try destruct_match eqn:enough_balance_check in new_balance; try congruence.
+    + (* case no contradictions *)
+      inversion_clear allowances_eq.
+      now inversion_clear new_balance.
+    + (* enough balances contradiction *)
+      receive_simpl.
+      apply N.ltb_lt in enough_balance_check.
+      now apply N.le_ngt in enough_balance.
+    + (* case: no contradictions *)
+      inversion_clear allowances_eq.
+      now inversion_clear new_balance.
+    + (* enough balances contradiction *)
+      receive_simpl.
+      apply N.ltb_lt in enough_balance_check.
+      now apply N.le_ngt in enough_balance.
+    + (* enough allowance contradiction *)
+      receive_simpl.
+      apply N.ltb_lt in enough_allowance_check.
+      destruct (address_eqb_spec ctx.(ctx_from) param.(from)) as [| sender_from_ne]; try discriminate.
+      now apply not_eq_sym, enough_allowance, N.le_ngt in sender_from_ne.
+  - intros (new_state & new_acts & receive_some).
+    receive_simpl.
+    split; try now apply Z.ltb_ge in ctx_amount_zero.
+    clear ctx_amount_zero g0.
+    rename H1 into enough_balance.
+    apply N.ltb_ge in enough_balance.
+    rename H into allowance_check.
+    destruct_match eqn:sender_from_eqb in allowance_check;
+      destruct (address_eqb_spec ctx.(ctx_from) param.(from)) as
+        [send_from_eq | sender_from_ne]; try discriminate.
+    + (* sender = from *)
+      now split.
+    + (* sender <> from *)
+      destruct_match eqn:enough_allowance in allowance_check; try congruence.
+      receive_simpl.
+      now apply N.ltb_ge in enough_allowance.
+Qed.
+
+
+
+(* ------------------- Approve correct ------------------- *)
+
+(* try_approve correctly sets allowance of (<sender>, <spender>) to <value_> *)
+Lemma try_approve_allowance_correct : forall prev_state new_state chain ctx new_acts param,
+  receive chain ctx prev_state (Some (msg_approve param)) = Some (new_state, new_acts) ->
+    FMap.find (ctx.(ctx_from), param.(spender)) (allowances new_state) = Some param.(value_).
+Proof.
+  intros * receive_some.
+  receive_simpl.
+  clear H ctx_amount_zero.
+  cbn.
+  now rewrite FMap.find_add.
+Qed.
+
+(* try_approve does not produce any new actions *)
+Lemma try_approve_new_acts_correct : forall prev_state new_state chain ctx new_acts param,
+  receive chain ctx prev_state (Some (msg_approve param)) = Some (new_state, new_acts) ->
+    new_acts = [].
+Proof.
+  intros * receive_some.
+  receive_simpl.
+Qed.
+
+(* try_approve does not change allowances map of other addresses *)
+Lemma try_approve_preserves_other_allowances : forall prev_state new_state chain ctx new_acts param,
+  receive chain ctx prev_state (Some (msg_approve param)) = Some (new_state, new_acts) ->
+    forall allowance_key, allowance_key <> (ctx.(ctx_from), param.(spender)) ->
+      FMap.find allowance_key (allowances prev_state) = FMap.find allowance_key (allowances new_state).
+Proof.
+  intros * receive_some allowance_key allowance_key_ne.
+  receive_simpl.
+  clear H ctx_amount_zero.
+  cbn.
+  now rewrite FMap.find_add_ne.
+Qed.
+
+(* try_approve does not change total supply of tokens *)
+Lemma try_approve_preserves_total_supply : forall prev_state new_state chain ctx new_acts param,
+  receive chain ctx prev_state (Some (msg_approve param)) = Some (new_state, new_acts) ->
+    total_supply prev_state = total_supply new_state.
+Proof.
+  intros * receive_some.
+  now receive_simpl.
+Qed.
+
+(* try_approve does not change balances *)
+Lemma try_approve_preserves_balances : forall prev_state new_state chain ctx new_acts param,
+  receive chain ctx prev_state (Some (msg_approve param)) = Some (new_state, new_acts) ->
+    tokens prev_state = tokens new_state.
+Proof.
+  intros * receive_some.
+  now receive_simpl.
+Qed.
+
+(* If the requirements are met then then receive on approve msg must succeed and
+    if receive on approve msg succeeds then requirements must hold *)
+Lemma try_approve_is_some : forall state chain ctx param,
+  (ctx_amount ctx <= 0)%Z /\
+  (with_default 0 (FMap.find (ctx.(ctx_from), param.(spender)) (allowances state)) = 0 \/ param.(value_) = 0)
+    <-> exists new_state new_acts, receive chain ctx state (Some (msg_approve param)) = Some (new_state, new_acts).
+Proof.
+  split.
+  - intros (amount_zero & safe_approval).
+    do 2 eexists.
+    receive_simpl.
+    apply Z.ltb_ge in amount_zero.
+    rewrite amount_zero.
+    destruct_match eqn:safe_approval_check; eauto.
+    receive_simpl.
+    apply andb_prop in safe_approval_check as
+      (?%N.ltb_lt & ?%N.ltb_lt).
+    now destruct safe_approval.
+  - intros (new_state & new_acts & receive_some).
+    receive_simpl.
+    split; try now apply Z.ltb_ge in ctx_amount_zero.
+    rename H into safe_approval.
+    now apply andb_false_iff in safe_approval as [?%N.ltb_ge | ?%N.ltb_ge].
+Qed.
+
+
+
+(* ------------------- Burn or mint correct ------------------- *)
+
+(* try_mint_or_burn correctly mints/burns <amount> from/to <target> *)
+Lemma try_mint_or_burn_balance_correct : forall prev_state new_state chain ctx new_acts param,
+  receive chain ctx prev_state (Some (msg_mint_or_burn param)) = Some (new_state, new_acts) ->
+    (Z.of_N (with_default 0%N (FMap.find param.(target) (tokens prev_state))) + param.(quantity) =
+    Z.of_N (with_default 0%N (FMap.find param.(target) (tokens new_state))))%Z.
+Proof.
+  intros * receive_some.
+  receive_simpl.
+  rename H0 into enough_tokens.
+  clear ctx_amount_zero H.
+  rewrite Z.ltb_ge in enough_tokens.
+  cbn.
+  rewrite FMap.find_add.
+  cbn.
+  now rewrite Z2N.id.
+Qed.
+
+(* try_mint_or_burn correctly updates total_supply *)
+Lemma try_mint_or_burn_total_supply_correct : forall prev_state new_state chain ctx new_acts param,
+  with_default 0 (FMap.find param.(target) (tokens prev_state)) <= total_supply prev_state ->
+  receive chain ctx prev_state (Some (msg_mint_or_burn param)) = Some (new_state, new_acts) ->
+    (Z.of_N prev_state.(total_supply) + param.(quantity) =
+    Z.of_N new_state.(total_supply))%Z.
+Proof.
+  intros * balance_le_total_supply receive_some.
+  receive_simpl.
+  rename H0 into enough_tokens.
+  clear ctx_amount_zero H.
+  rewrite Z.ltb_ge in enough_tokens.
+  cbn.
+  rewrite N2Z.inj_abs_N, Z.abs_eq; auto.
+  eapply Z.le_trans; try apply enough_tokens.
+  now apply Zplus_le_compat_r, N2Z.inj_le.
+Qed.
+
+
+(* try_mint_or_burn produces no new actions *)
+Lemma try_mint_or_burn_new_acts_correct : forall prev_state new_state chain ctx new_acts param,
+  receive chain ctx prev_state (Some (msg_mint_or_burn param)) = Some (new_state, new_acts) ->
+    new_acts = [].
+Proof.
+  intros.
+  receive_simpl.
+Qed.
+
+(* try_mint_or_burn only modifies the <target> balance *)
+Lemma try_mint_or_burn_preserves_other_balances : forall prev_state new_state chain ctx new_acts param,
+  receive chain ctx prev_state (Some (msg_mint_or_burn param)) = Some (new_state, new_acts) ->
+    forall account, account <> param.(target) ->
+      FMap.find account (tokens prev_state) = FMap.find account (tokens new_state).
+Proof.
+  intros * receive_some account account_not_target.
+  receive_simpl.
+  cbn.
+  rewrite FMap.find_add_ne; auto.
+Qed.
+
+(* try_mint_or_burn does not change allowances *)
+Lemma try_mint_or_burn_preserves_allowances : forall prev_state new_state chain ctx new_acts param,
+  receive chain ctx prev_state (Some (msg_mint_or_burn param)) = Some (new_state, new_acts) ->
+      allowances prev_state = allowances new_state.
+Proof.
+  intros * receive_some.
+  now receive_simpl.
+Qed.
+
+(* If the requirements are met then then receive on mint_or_burn msg must succeed and
+    if receive on mint_or_burn msg succeeds then requirements must hold *)
+Lemma try_mint_or_burn_is_some : forall state chain ctx param,
+  (ctx_amount ctx <= 0)%Z /\
+  ctx.(ctx_from) = state.(admin) /\
+  (0 <= Z.of_N (with_default 0%N (FMap.find param.(target) (tokens state))) + param.(quantity))%Z
+    <-> exists new_state new_acts, receive chain ctx state (Some (msg_mint_or_burn param)) = Some (new_state, new_acts).
+Proof.
+  split.
+  - intros (amount_zero & from_admin & enough_balance).
+    do 2 eexists.
+    receive_simpl.
+    apply Z.ltb_ge in amount_zero.
+    rewrite amount_zero.
+    destruct_address_eq; try congruence.
+    clear e from_admin. cbn.
+    destruct_match eqn:enough_balance_check; eauto.
+    receive_simpl.
+    now apply Z.ltb_lt in enough_balance_check.
+  - intros (new_state & new_acts & receive_some).
+    receive_simpl.
+    split; try now apply Z.ltb_ge in ctx_amount_zero.
+    split; try now destruct_address_eq.
+    now apply Z.ltb_ge.
+Qed.
+
+
+
+(* ------------------- Get allowance correct ------------------- *)
+
+(* try_get_allowance produces a callback to the correct contract with
+    the requested allowance, the call should carry no balance *)
+Lemma try_get_allowance_new_acts_correct : forall prev_state new_state chain ctx new_acts param,
+  receive chain ctx prev_state (Some (msg_get_allowance param)) = Some (new_state, new_acts) ->
+    new_acts = [
+      act_call ctx.(ctx_from) 0%Z (serialize
+        (receive_allowance (with_default 0 (FMap.find param.(request) (allowances prev_state)))))
+    ].
+Proof.
+  intros * receive_some.
+  now receive_simpl.
+Qed.
+
+(* try_get_allowance does not modify state *)
+Lemma try_get_allowance_preserves_state : forall prev_state new_state chain ctx new_acts param,
+  receive chain ctx prev_state (Some (msg_get_allowance param)) = Some (new_state, new_acts) ->
+    prev_state = new_state.
+Proof.
+  intros * receive_some.
+  now receive_simpl.
+Qed.
+
+(* If the requirements are met then then receive on get_allowance msg must succeed and
+    if receive on get_allowance msg succeeds then requirements must hold *)
+Lemma try_get_allowance_is_some : forall prev_state chain ctx param,
+  (ctx_amount ctx <= 0)%Z <->
+  exists new_state new_acts, receive chain ctx prev_state (Some (msg_get_allowance param)) = Some (new_state, new_acts).
+Proof.
+  split.
+  - intros amount_zero.
+    unfold receive.
+    apply Z.ltb_ge in amount_zero.
+    now rewrite amount_zero.
+  - intros (new_state & new_acts & receive_some).
+    receive_simpl.
+    now apply Z.ltb_ge in ctx_amount_zero.
+Qed.
+
+
+
+(* ------------------- Get balance correct ------------------- *)
+
+(* try_get_balance produces a callback to the correct contract with
+    the requested balance, the call should carry no balance *)
+Lemma try_get_balance_new_acts_correct : forall prev_state new_state chain ctx new_acts param,
+  receive chain ctx prev_state (Some (msg_get_balance param)) = Some (new_state, new_acts) ->
+    new_acts = [
+      act_call ctx.(ctx_from) 0%Z (serialize
+        (receive_balance_of (with_default 0 (FMap.find param.(owner_) (tokens prev_state)))))
+    ].
+Proof.
+  intros * receive_some.
+  now receive_simpl.
+Qed.
+
+(* try_get_balance does not modify state *)
+Lemma try_get_balance_preserves_state : forall prev_state new_state chain ctx new_acts param,
+  receive chain ctx prev_state (Some (msg_get_balance param)) = Some (new_state, new_acts) ->
+    prev_state = new_state.
+Proof.
+  intros * receive_some.
+  now receive_simpl.
+Qed.
+
+(* If the requirements are met then then receive on get_balance msg must succeed and
+    if receive on get_balance msg succeeds then requirements must hold *)
+Lemma try_get_balance_is_some : forall prev_state chain ctx param,
+  (ctx_amount ctx <= 0)%Z <->
+  exists new_state new_acts, receive chain ctx prev_state (Some (msg_get_balance param)) = Some (new_state, new_acts).
+Proof.
+  split.
+  - intros amount_zero.
+    unfold receive.
+    apply Z.ltb_ge in amount_zero.
+    now rewrite amount_zero.
+  - intros (new_state & new_acts & receive_some).
+    receive_simpl.
+    now apply Z.ltb_ge in ctx_amount_zero.
+Qed.
+
+
+
+(* ------------------- Get total supply correct ------------------- *)
+
+(* try_get_total_supply produces a callback to the correct contract with
+    the tptal supply of tokens, the call should carry no balance *)
+Lemma try_get_total_supply_new_acts_correct : forall prev_state new_state chain ctx new_acts param,
+  receive chain ctx prev_state (Some (msg_get_total_supply param)) = Some (new_state, new_acts) ->
+    new_acts = [
+      act_call ctx.(ctx_from) 0%Z (serialize
+        (receive_total_supply prev_state.(total_supply)))
+    ].
+Proof.
+  intros * receive_some.
+  now receive_simpl.
+Qed.
+
+(* try_get_total_supply does not modify state *)
+Lemma try_get_total_supply_preserves_state : forall prev_state new_state chain ctx new_acts param,
+  receive chain ctx prev_state (Some (msg_get_total_supply param)) = Some (new_state, new_acts) ->
+    prev_state = new_state.
+Proof.
+  intros * receive_some.
+  now receive_simpl.
+Qed.
+
+(* If the requirements are met then then receive on get_total_supply msg must succeed and
+    if receive on get_total_supply msg succeeds then requirements must hold *)
+Lemma try_get_total_supply_is_some : forall prev_state chain ctx param,
+  (ctx_amount ctx <= 0)%Z <->
+  exists new_state new_acts, receive chain ctx prev_state (Some (msg_get_total_supply param)) = Some (new_state, new_acts).
+Proof.
+  split.
+  - intros amount_zero.
+    unfold receive.
+    apply Z.ltb_ge in amount_zero.
+    now rewrite amount_zero.
+  - intros (new_state & new_acts & receive_some).
+    receive_simpl.
+    now apply Z.ltb_ge in ctx_amount_zero.
+Qed.
+
+
+
+(* ------------------- Init correct ------------------- *)
+
+(* After initalization no accounts should hold tokens *)
+Lemma init_balances_correct : forall chain ctx setup state,
+  init chain ctx setup = Some state ->
+    state.(tokens) = FMap.add setup.(lqt_provider) setup.(initial_pool) FMap.empty.
+Proof.
+  intros * init_some.
+  now inversion init_some.
+Qed.
+
+(* After initalization no allowances should be set *)
+Lemma init_allowances_correct : forall chain ctx setup state,
+  init chain ctx setup = Some state ->
+    state.(allowances) = FMap.empty.
+Proof.
+  intros * init_some.
+  now inversion init_some.
+Qed.
+
+Lemma init_admin_correct : forall chain ctx setup state,
+  init chain ctx setup = Some state ->
+    state.(admin) = setup.(admin_).
+Proof.
+  intros * init_some.
+  now inversion init_some.
+Qed.
+
+Lemma init_total_supply_correct : forall chain ctx setup state,
+  init chain ctx setup = Some state ->
+    state.(total_supply) = setup.(initial_pool).
+Proof.
+  intros * init_some.
+  now inversion init_some.
+Qed.
+
+(* initialization should always succeed *)
+Lemma init_is_some : forall chain ctx setup,
+  exists state, init chain ctx setup = state.
+Proof.
+  intros.
+  eauto.
+Qed.
+
+
+
+(* ------------------- Outgoing acts facts ------------------- *)
+
+(* contract never calls itself *)
+Lemma no_self_calls bstate caddr :
+  reachable bstate ->
+  env_contracts bstate caddr = Some (contract : WeakContract) ->
+  Forall (fun act_body =>
+    match act_body with
+    | act_transfer to _
+    | act_call to _ _ => (to =? caddr)%address = false
+    | _ => False
+    end) (outgoing_acts bstate caddr).
+Proof.
+  contract_induction; intros; auto.
+  - now inversion IH.
+  - apply Forall_app; split; auto.
+    clear IH.
+    destruct msg. destruct m.
+    + now erewrite try_transfer_new_acts_correct by eauto.
+    + now erewrite try_approve_new_acts_correct by eauto.
+    + now erewrite try_mint_or_burn_new_acts_correct by eauto.
+    + erewrite try_get_allowance_new_acts_correct by eauto.
+      constructor; auto.
+      now destruct_address_eq.
+    + erewrite try_get_balance_new_acts_correct by eauto.
+      constructor; auto.
+      now destruct_address_eq.
+    + erewrite try_get_total_supply_new_acts_correct by eauto.
+      constructor; auto.
+      now destruct_address_eq.
+    + now rewrite default_entrypoint_none in receive_some.
+  - inversion_clear IH as [|? ? head_not_me tail_not_me].
+    destruct head;
+      try contradiction;
+      destruct action_facts;
+      subst;
+      now rewrite address_eq_refl in head_not_me.
+  - now rewrite <- perm.
+  - instantiate (AddBlockFacts := fun _ _ _ _ _ _ => True).
+    instantiate (DeployFacts := fun _ _ => True).
+    instantiate (CallFacts := fun _ _ _ _ => True).
+    unset_all; subst;cbn in *.
+    destruct_chain_step; auto.
+    destruct_action_eval; auto.
+Qed.
+
+Lemma no_self_calls' : forall bstate from_addr to_addr amount msg acts,
+  reachable bstate ->
+  env_contracts bstate to_addr = Some (contract : WeakContract) ->
+  chain_state_queue bstate = {| act_from := from_addr; act_body :=
+    match msg with
+    | Some msg => act_call to_addr amount msg
+    | None => act_transfer to_addr amount
+    end |} :: acts ->
+  from_addr <> to_addr.
+Proof.
+  intros * reach deployed queue.
+  apply no_self_calls in deployed as no_self_calls; auto.
+  unfold outgoing_acts in no_self_calls.
+  rewrite queue in no_self_calls.
+  cbn in no_self_calls.
+  destruct_address_eq; auto.
+  inversion_clear no_self_calls as [|? ? hd _].
+  destruct msg;
+    now rewrite address_eq_refl in hd.
+Qed.
+
+Lemma new_acts_amount_zero : forall prev_state chain ctx msg new_state new_acts,
+  receive chain ctx prev_state msg = Some (new_state, new_acts) ->
+    sumZ (fun act => act_body_amount act) new_acts = 0%Z.
+Proof.
+  intros * receive_some.
+  destruct msg. destruct m.
+  - apply try_transfer_new_acts_correct in receive_some.
+    now subst.
+  - apply try_approve_new_acts_correct in receive_some.
+    now subst.
+  - apply try_mint_or_burn_new_acts_correct in receive_some.
+    now subst.
+  - apply try_get_allowance_new_acts_correct in receive_some.
+    now subst.
+  - apply try_get_balance_new_acts_correct in receive_some.
+    now subst.
+  - apply try_get_total_supply_new_acts_correct in receive_some.
+    now subst.
+  - now rewrite default_entrypoint_none in receive_some.
+Qed.
+
+Lemma outgoing_acts_amount_zero : forall bstate caddr,
+  reachable bstate ->
+  env_contracts bstate caddr = Some (contract : WeakContract) ->
+  Forall (fun act => act_body_amount act = 0%Z) (outgoing_acts bstate caddr).
+Proof.
+  intros * reach deployed.
+  apply (lift_outgoing_acts_prop contract); auto.
+  intros * receive_some.
+  destruct msg. destruct m.
+  - apply try_transfer_new_acts_correct in receive_some.
+    now subst.
+  - apply try_approve_new_acts_correct in receive_some.
+    now subst.
+  - apply try_mint_or_burn_new_acts_correct in receive_some.
+    now subst.
+  - apply try_get_allowance_new_acts_correct in receive_some.
+    now subst.
+  - apply try_get_balance_new_acts_correct in receive_some.
+    now subst.
+  - apply try_get_total_supply_new_acts_correct in receive_some.
+    now subst.
+  - now rewrite default_entrypoint_none in receive_some.
+Qed.
+
+(* contract only produces call acts *)
+Lemma outgoing_acts_are_calls : forall bstate caddr,
+  reachable bstate ->
+  env_contracts bstate caddr = Some (contract : WeakContract) ->
+  Forall (fun act_body =>
+    match act_body with
+    | act_call _ _ _ => True
+    | _ => False
+    end) (outgoing_acts bstate caddr).
+Proof.
+  intros * reach deployed.
+  apply (lift_outgoing_acts_prop contract); auto.
+  intros * receive_some.
+  destruct msg. destruct m.
+  - apply try_transfer_new_acts_correct in receive_some.
+    now subst.
+  - apply try_approve_new_acts_correct in receive_some.
+    now subst.
+  - apply try_mint_or_burn_new_acts_correct in receive_some.
+    now subst.
+  - apply try_get_allowance_new_acts_correct in receive_some.
+    now subst.
+  - apply try_get_balance_new_acts_correct in receive_some.
+    now subst.
+  - apply try_get_total_supply_new_acts_correct in receive_some.
+    now subst.
+  - now rewrite default_entrypoint_none in receive_some.
+Qed.
+
+
+(* ------------------- Contract balance facts ------------------- *)
+
+(* Contract balance should never change and thus always be equal to the deploy amount *)
+Lemma contract_balance_bound' : forall bstate caddr (trace : ChainTrace empty_state bstate),
+  let effective_balance := (env_account_balances bstate caddr - (sumZ (fun act => act_body_amount act) (outgoing_acts bstate caddr)))%Z in
+  env_contracts bstate caddr = Some (contract : WeakContract) ->
+  exists deploy_info,
+    deployment_info Setup trace caddr = Some deploy_info
+    /\ effective_balance = deploy_info.(deployment_amount).
+Proof.
+  intros.
+  unfold effective_balance.
+  contract_induction; intros; auto.
+  - cbn.
+    lia.
+  - cbn in IH.
+    lia.
+  - instantiate (CallFacts := fun _ ctx _ _ =>
+      (0 <= ctx_amount ctx)%Z /\ ctx_from ctx <> ctx_contract_address ctx).
+    destruct facts as (ctx_amount_positive & _).
+    apply contract_not_payable in receive_some as not_payable.
+    apply new_acts_amount_zero in receive_some as amount_zero_new_acts.
+    apply Z.le_antisymm in ctx_amount_positive; auto.
+    rewrite ctx_amount_positive, Z.sub_0_r in IH.
+    now rewrite sumZ_app, amount_zero_new_acts, Z.add_0_l.
+  - now destruct facts.
+  - now erewrite sumZ_permutation in IH by eauto.
+  - instantiate (AddBlockFacts := fun _ _ _ _ _ _ => True).
+    instantiate (DeployFacts := fun _ _ => True).
+    unset_all; subst.
+    destruct_chain_step; auto.
+    destruct_action_eval; auto.
+    intros cstate contract_deployed deployed_state.
+    subst. cbn.
+    split.
+    + now apply Z.ge_le.
+    + now eapply no_self_calls'.
+Qed.
+
+Lemma contract_balance_bound : forall bstate caddr (trace : ChainTrace empty_state bstate),
+  env_contracts bstate caddr = Some (contract : WeakContract) ->
+  exists deploy_info,
+    deployment_info Setup trace caddr = Some deploy_info
+    /\ env_account_balances bstate caddr = deploy_info.(deployment_amount).
+Proof.
+  intros * deployed.
+  specialize contract_balance_bound' as (dep_info & deployment_info_eq & balance_bound); eauto.
+  eexists.
+  rewrite deployment_info_eq.
+  split; eauto.
+  rewrite <- balance_bound.
+  rewrite Zminus_0_l_reverse, Z.sub_cancel_l at 1.
+  apply outgoing_acts_amount_zero in deployed as act_amount_zero;
+    try now constructor.
+  clear balance_bound deployment_info_eq dep_info trace deployed.
+  induction (outgoing_acts bstate caddr).
+  - reflexivity.
+  - cbn.
+    apply list.Forall_cons in act_amount_zero as (act_amount_zero & acts_amount_zero).
+    rewrite act_amount_zero, Z.add_0_l.
+    now apply IHl.
+Qed.
+
+
+
+(* ------------------- Total supply / token balance facts ------------------- *)
+
+(* sum of all token balances *)
+Definition sum_balances state :=
+  sumN (fun '(k, v) => v) (FMap.elements (tokens state)).
+
+(* The balance of a single account is always less than
+   or equal to the sum of all balances *)
+Lemma balance_le_sum_balances : forall addr state,
+  with_default 0 (FMap.find addr (tokens state)) <= sum_balances state.
+Proof.
+  intros.
+  destruct FMap.find eqn:balance.
+  - eapply FMap.In_elements, sumN_in_le in balance.
+    eapply N.le_trans; cycle 1; eauto.
+  - apply N.le_0_l.
+Qed.
+
+Lemma sum_balances_eq_total_supply : forall bstate caddr,
+  reachable bstate ->
+  env_contracts bstate caddr = Some (contract : WeakContract) ->
+  exists cstate,
+    contract_state bstate caddr = Some cstate
+    /\ total_supply cstate = sum_balances cstate.
+Proof.
+  contract_induction; intros; auto.
+  - unfold sum_balances.
+    erewrite init_total_supply_correct, init_balances_correct; eauto.
+    rewrite FMap.elements_add, FMap.elements_empty by auto.
+    now cbn.
+  - destruct msg. destruct m.
+    + erewrite <- try_transfer_preserves_total_supply; eauto.
+      rename t into param.
+      unfold sum_balances.
+      receive_simpl.
+      cbn.
+      rename H1 into enough_balance.
+      apply N.ltb_ge in enough_balance.
+      clear tag ctx_amount_zero g g0 H facts from_other new_acts new_state dep_info ctx
+          prev_out_queue prev_inc_calls prev_out_txs trace caddr AddBlockFacts DeployFacts
+          CallFacts chain bstate.
+      destruct (address_eqb_spec param.(from) param.(to)) as
+        [<-| from_to_ne];
+        destruct (FMap.find (from param) (tokens prev_state)) eqn:from_balance;
+        destruct (FMap.find (to param) (tokens prev_state)) eqn:to_balance;
+          cbn in enough_balance;
+          repeat match goal with
+            | H : ?x = ?y |- context [ ?x ] => rewrite H
+            | H : _ <= 0 |- _ => apply N.lt_eq_cases in H as [H | H]; try lia; subst
+            | |- context [ FMap.find ?x (FMap.add ?x _ _) ] => rewrite FMap.find_add
+            | |- context [ FMap.add ?x _ (FMap.add ?x _ _) ] => rewrite FMap.add_add
+            | H : ?x <> ?y |- context [ FMap.find ?x (FMap.add ?y _ _) ] => rewrite FMap.find_add_ne; eauto
+            | H : ?y <> ?x |- context [ FMap.find ?x (FMap.add ?y _ _) ] => rewrite FMap.find_add_ne; eauto
+            | H : FMap.find ?x _ = Some _ |- context [ FMap.elements (FMap.add ?x _ _) ] => rewrite FMap.elements_add_existing; eauto
+            | H : FMap.find ?x _ = None |- context [ FMap.elements (FMap.add ?x _ _) ] => rewrite FMap.elements_add; eauto
+            | |- context [ FMap.remove ?x (FMap.add ?x _ _) ] => rewrite fin_maps.delete_insert_delete
+            | H : FMap.find ?x ?m = Some _ |- context [ sumN _ ((_, _) :: FMap.elements (FMap.remove ?x ?m)) ] => rewrite fin_maps.map_to_list_delete; auto
+            | H : FMap.find ?x _ = Some ?n |- context [ sumN _ ((?x, ?n) :: (_, _) :: FMap.elements (FMap.remove ?x _)) ] => rewrite sumN_swap, fin_maps.map_to_list_delete; auto
+            | |- context [ sumN _ ((?t, ?n + ?m) :: _) ] => erewrite sumN_split with (x:= (t, n)) (y := (_, m)) by lia
+            | |- context [ sumN _ ((_, 0) :: (?x, ?n) :: _) ] => erewrite <- sumN_split with (z := (x, n)) by auto
+            | |- context [ sumN _ ((_, ?n) :: (?x, ?m - ?n) :: _) ] => erewrite <- sumN_split with (z := (x, n + m - n))
+            | |- context [ sumN _ ((?x, ?m - ?n) :: (_, ?n) :: _) ] => erewrite <- sumN_split with (z := (x, n + m - n))
+            | |- context [ with_default _ None ] => unfold with_default
+            | |- context [ with_default _ (Some _) ] => unfold with_default
+           end; try easy.
+    + erewrite <- try_approve_preserves_total_supply; eauto.
+      unfold sum_balances.
+      erewrite <- try_approve_preserves_balances; eauto.
+    + rename m into param.
+      unfold sum_balances.
+      receive_simpl.
+      cbn.
+      clear tag ctx_amount_zero H facts from_other new_acts new_state dep_info ctx
+          prev_out_queue prev_inc_calls prev_out_txs trace caddr AddBlockFacts DeployFacts
+          CallFacts chain bstate.
+      rename H0 into enough_balance.
+      apply Z.ltb_ge in enough_balance.
+      destruct (FMap.find (target param) (tokens prev_state)) eqn:target_balance; cbn.
+      * specialize (balance_le_sum_balances param.(target) prev_state) as n_le_supply.
+        rewrite target_balance in n_le_supply.
+        cbn in n_le_supply.
+        rewrite FMap.elements_add_existing by eauto.
+        cbn.
+        rewrite N.add_comm.
+        assert (N_add_sub_move : forall n m p, p <= n -> n - p = m -> n = m + p) by lia.
+        apply N_add_sub_move; try lia.
+        rewrite <- Zabs2N.abs_N_nonneg by assumption.
+        rewrite <- Zabs2N.inj_sub by (split; [assumption | lia]).
+        rewrite Z.add_add_simpl_r_r, Zabs2N.inj_sub, !Zabs2N.id by lia.
+        apply N.add_sub_eq_r.
+        change n with ((fun '(_, v) => v) (target param, n)).
+        now rewrite sumN_inv, fin_maps.map_to_list_delete by assumption.
+      * rewrite FMap.elements_add by auto. cbn.
+        unfold sum_balances in IH.
+        rewrite <- IH.
+        now rewrite <- Zabs2N.id, N2Z.inj_add, Z2N.id.
+    + now apply try_get_allowance_preserves_state in receive_some.
+    + now apply try_get_balance_preserves_state in receive_some.
+    + now apply try_get_total_supply_preserves_state in receive_some.
+    + now rewrite default_entrypoint_none in receive_some.
+  - now instantiate (CallFacts := fun _ ctx _ _ =>  ctx_from ctx <> ctx_contract_address ctx).
+  - instantiate (AddBlockFacts := fun _ _ _ _ _ _ => True).
+    instantiate (DeployFacts := fun _ _ => True).
+    unset_all; subst.
+    destruct_chain_step; auto.
+    destruct_action_eval; auto.
+    intros.
+    subst. cbn.
+    now eapply no_self_calls'.
+  Unshelve. all : destruct param; eauto.
+Qed.
+
+Lemma token_balance_le_total_supply : forall bstate caddr,
+  reachable bstate ->
+  env_contracts bstate caddr = Some (contract : WeakContract) ->
+  exists cstate,
+    contract_state bstate caddr = Some cstate
+    /\ forall addr, with_default 0 (FMap.find addr (tokens cstate)) <= total_supply cstate.
+Proof.
+  intros * reach deployed.
+  apply sum_balances_eq_total_supply in deployed as
+    (cstate & deployed_state & sum_eq_supply); auto.
+  eexists.
+  rewrite deployed_state, sum_eq_supply.
+  clear reach deployed_state sum_eq_supply caddr bstate.
+  split; auto.
+  intros.
+  apply balance_le_sum_balances.
+Qed.
+
+End Theories.
 End LQTFA12.
